implemented and verified a few functions from IMP- Max Constant

IMP-/IMP_Minus_Nat_Bijection.thy
@@ -5,6 +5,8 @@ theory IMP_Minus_Nat_Bijection
     "../Cook_Levin/IMP-_To_SAS+/IMP-_To_IMP--/Primitives"
 begin
 
+unbundle IMP_Minus_Minus_Com.no_com_syntax
+
 definition IMP_Minus_triangle where "IMP_Minus_triangle \<equiv>
   ''b'' ::= ((V ''a'') \<oplus> (N 1)) ;;
   IMP_minus_mul ;;
@@ -104,14 +106,17 @@ definition IMP_Minus_fst_nat where "IMP_Minus_fst_nat \<equiv>
   ''a'' ::= (A (N 0)) ;;
   ''b'' ::= (A (N 0))"
 
+definition IMP_Minus_fst_nat_time where "IMP_Minus_fst_nat_time x \<equiv>
+  14 + 7 * prod_decode_aux_iterations 0 x"
+
 lemma IMP_Minus_fst_nat_correct: 
   "(IMP_Minus_fst_nat, s) 
-      \<Rightarrow>\<^bsup>14 + 7 * prod_decode_aux_iterations 0 (s ''a'')\<^esup> 
+      \<Rightarrow>\<^bsup>IMP_Minus_fst_nat_time (s ''a'')\<^esup> 
     s(''a'' := 0,
       ''b'' := 0,
       ''c'' := 0,
       ''fst_nat'' := fst_nat (s ''a''))"
-  unfolding IMP_Minus_fst_nat_def fst_nat_def prod_decode_def
+  unfolding IMP_Minus_fst_nat_def fst_nat_def prod_decode_def IMP_Minus_fst_nat_time_def
   by (force intro!: 
       terminates_in_state_intro[OF Seq]
       prod_decode_aux_loop_correct)
@@ -127,13 +132,98 @@ definition IMP_Minus_snd_nat where "IMP_Minus_snd_nat \<equiv>
 
 lemma IMP_Minus_snd_nat_correct: 
   "(IMP_Minus_snd_nat, s) 
-      \<Rightarrow>\<^bsup>14 + 7 * prod_decode_aux_iterations 0 (s ''a'')\<^esup> 
+      \<Rightarrow>\<^bsup>IMP_Minus_fst_nat_time (s ''a'')\<^esup> 
     s(''a'' := 0,
       ''b'' := 0,
       ''c'' := 0,
       ''snd_nat'' := snd_nat (s ''a''))"
-  unfolding IMP_Minus_snd_nat_def snd_nat_def prod_decode_def
+  unfolding IMP_Minus_snd_nat_def snd_nat_def prod_decode_def IMP_Minus_fst_nat_time_def
   by (force intro!: 
       terminates_in_state_intro[OF Seq]
       prod_decode_aux_loop_correct)
+
+definition nth_nat_iteration where "nth_nat_iteration \<equiv>
+  ''a'' ::= ((V ''a'') \<ominus> (N 1)) ;;
+  IMP_Minus_snd_nat ;;
+  ''a'' ::= (A (V ''snd_nat'')) ;;
+  ''snd_nat'' ::= (A (N 0)) ;;
+  ''nth_nat'' ::= ((V ''nth_nat'') \<ominus> (N 1))"
+
+fun nth_nat_loop_time :: "nat \<Rightarrow> nat \<Rightarrow> nat" where
+"nth_nat_loop_time 0 x = 2" |
+"nth_nat_loop_time (Suc n) x = 9 + IMP_Minus_fst_nat_time (x - 1) 
+  + nth_nat_loop_time n (tl_nat x)"
+
+fun drop_n_nat :: "nat \<Rightarrow> nat\<Rightarrow> nat" where 
+"drop_n_nat 0 x = x "|
+"drop_n_nat (Suc n) x = drop_n_nat n (tl_nat x)"
+
+lemma nth_nat_is_hd_of_drop_n_nat:
+  "nth_nat n x = fst_nat (drop_n_nat n x - Suc 0)"
+  by (induction n arbitrary: x)
+    (auto simp: hd_nat_def)
+
+lemma nth_nat_loop_correct:
+  "s ''nth_nat'' = k
+  \<Longrightarrow> (WHILE ''nth_nat'' \<noteq>0 DO nth_nat_iteration, s) 
+      \<Rightarrow>\<^bsup>nth_nat_loop_time (s ''nth_nat'') (s ''a'') \<^esup>
+      s(''a'' := drop_n_nat k (s ''a''),
+        ''b'' := (if k > 0 then 0 else s ''b''),
+        ''c'' := (if k > 0 then 0 else s ''c''),
+        ''snd_nat'' := (if k > 0 then 0 else s ''snd_nat''),
+        ''nth_nat'' := 0)"
+proof(induction k arbitrary: s)
+  case 0
+  then show ?case
+    by(auto simp: numeral_eq_Suc fun_eq_iff 
+        intro!: terminates_in_state_intro[OF Big_StepT.WhileFalse])
+next
+  case (Suc k)
+
+  have first_iteration: "(nth_nat_iteration, s)
+    \<Rightarrow>\<^bsup> 8 + IMP_Minus_fst_nat_time ((s ''a'') - 1) \<^esup>
+      s(''a'' := tl_nat (s ''a''),
+        ''b'' := 0,
+        ''c'' := 0,
+        ''snd_nat'' := 0,
+        ''nth_nat'' := k)"
+    unfolding nth_nat_iteration_def tl_nat_def
+    using \<open>s ''nth_nat'' = Suc k\<close>
+    by(force intro!: terminates_in_state_intro[OF Seq]
+        IMP_Minus_snd_nat_correct)
+
+  show ?case
+    using \<open>s ''nth_nat'' = Suc k\<close>
+    by (force intro!: terminates_in_state_intro
+          [OF Big_StepT.WhileTrue[OF _ first_iteration Suc.IH]])
+qed
+
+
+definition nth_nat_IMP_Minus where "nth_nat_IMP_Minus \<equiv>
+  ''nth_nat'' ::= (A (V ''a'')) ;;
+  ''a'' ::= (A (V ''b'')) ;;
+  WHILE ''nth_nat'' \<noteq>0 DO nth_nat_iteration ;;
+  ''snd_nat'' ::= (A (N 0)) ;;
+  ''a'' ::= ((V ''a'') \<ominus> (N 1)) ;;
+  IMP_Minus_fst_nat ;;
+  ''nth_nat'' ::= (A (V ''fst_nat'')) ;;
+  ''fst_nat'' ::= (A (N 0))"
+
+definition nth_nat_IMP_Minus_time where "nth_nat_IMP_Minus_time n x \<equiv>
+  12 + nth_nat_loop_time n x + IMP_Minus_fst_nat_time ((drop_n_nat n x) - 1)"
+
+lemma nth_nat_IMP_Minus_correct:
+  "(nth_nat_IMP_Minus, s) \<Rightarrow>\<^bsup>nth_nat_IMP_Minus_time (s ''a'') (s ''b'') \<^esup>
+    s(''a'' := 0,
+      ''b'' := 0,
+      ''c'' := 0,
+      ''fst_nat'' := 0,
+      ''snd_nat'' := 0,
+      ''nth_nat'' := nth_nat (s ''a'') (s ''b''))"
+  apply(cases "s ''a'' = 0")
+  unfolding nth_nat_IMP_Minus_def nth_nat_IMP_Minus_time_def tl_nat_def 
+  by (fastforce simp: hd_nat_def nth_nat_is_hd_of_drop_n_nat
+            intro!: terminates_in_state_intro[OF Seq] 
+              IMP_Minus_fst_nat_correct nth_nat_loop_correct)+
+
 end
