Cook_Levin/IMP-_To_SAS+/IMP_Minus_Max_Constant_IMP_Minus.thy
@@ -1,0 +1,141 @@
+theory IMP_Minus_Max_Constant_IMP_Minus
+  imports IMP_Minus_Max_Constant_Nat
+    "../../IMP-/IMP_Minus_Nat_Bijection"
+begin
+
+unbundle IMP_Minus_Minus_Com.no_com_syntax
+
+definition atomExp_to_constant_IMP_Minus where "atomExp_to_constant_IMP_Minus \<equiv>
+  ''atomExp_to_constant'' ::= (A (V ''a'')) ;;
+  IMP_Minus_fst_nat ;;
+  ''a'' ::= (A (V ''atomExp_to_constant'')) ;;
+  IMP_Minus_snd_nat ;;
+  (IF ''fst_nat'' \<noteq>0 
+  THEN 
+    ''atomExp_to_constant'' ::= (A (V ''snd_nat''))  
+  ELSE
+    ''atomExp_to_constant'' ::=  (A (N 0)));;
+  ''fst_nat'' ::= (A (N 0)) ;;
+  ''snd_nat'' ::= (A (N 0))"
+
+definition atomExp_to_constant_IMP_Minus_time where "atomExp_to_constant_IMP_Minus_time x \<equiv>
+  11 + 2 * IMP_Minus_fst_nat_time x"
+
+lemma atomExp_to_constant_IMP_Minus_correct:
+  "(atomExp_to_constant_IMP_Minus, s) \<Rightarrow>\<^bsup>atomExp_to_constant_IMP_Minus_time (s ''a'')\<^esup> 
+    s(''a'' := 0,
+      ''b'' := 0,
+      ''c'' := 0,
+      ''fst_nat'' := 0,
+      ''snd_nat'' := 0,
+      ''atomExp_to_constant'' := atomExp_to_constant_tail (s ''a''))"
+  apply(cases "fst_nat (s ''a'')")
+  unfolding atomExp_to_constant_IMP_Minus_def atomExp_to_constant_tail_def
+    atomExp_to_constant_nat_def atomExp_to_constant_IMP_Minus_time_def
+  by (fastforce 
+      intro!: terminates_in_state_intro[OF Seq]
+      IMP_Minus_fst_nat_correct      
+      IMP_Minus_snd_nat_correct)+
+
+definition aexp_max_constant_IMP_Minus where "aexp_max_constant_IMP_Minus \<equiv> 
+  ''aexp_max_constant'' ::= (A (V ''a'')) ;;
+
+  ''a'' ::= (A (N 1)) ;;
+  ''b'' ::= (A (V ''aexp_max_constant'')) ;;
+  nth_nat_IMP_Minus ;;
+  
+  ''a'' ::= (A (V ''nth_nat'')) ;;
+  atomExp_to_constant_IMP_Minus ;;
+  
+  ''a'' ::= (A (N 2)) ;;
+  ''b'' ::= (A (V ''aexp_max_constant'')) ;;
+  nth_nat_IMP_Minus ;;
+  
+  ''a'' ::= (A (V ''nth_nat'')) ;;
+  ''nth_nat'' ::= (A (V ''atomExp_to_constant'')) ;;
+  atomExp_to_constant_IMP_Minus ;;
+
+  ''a'' ::= ((V ''aexp_max_constant'') \<ominus> (N 1)) ;;
+  IMP_Minus_fst_nat ;;
+
+  ''a'' ::= ((N 3) \<ominus> (V ''fst_nat'')) ;;
+  IF ''a'' \<noteq>0 
+  THEN
+  (
+    IF ''fst_nat'' \<noteq>0
+    THEN
+      ''b'' ::= (A (V ''atomExp_to_constant''))
+    ELSE
+      ''b'' ::= (A (V ''nth_nat''))
+  )
+  ELSE
+  (
+    IF ''fst_nat'' \<noteq>0
+    THEN
+      ''b'' ::= (A (V ''nth_nat''))
+    ELSE
+      ''b'' ::= (A (V ''nth_nat''))
+  );;
+
+  ''a'' ::= (A (V ''nth_nat'')) ;;
+
+  IMP_Minus_max_a_min_b ;;
+  ''aexp_max_constant'' ::= (A (V ''a'')) ;;
+  ''a'' ::= (A (N 0)) ;; 
+  ''b'' ::= (A (N 0)) ;;
+  ''nth_nat'' ::= (A (N 0)) ;;
+  ''atomExp_to_constant'' ::= (A (N 0)) ;;
+  ''fst_nat'' ::= (A (N 0))"
+
+definition aexp_max_constant_IMP_Minus_time where "aexp_max_constant_IMP_Minus_time x \<equiv>
+  38 + nth_nat_IMP_Minus_time 1 x + atomExp_to_constant_IMP_Minus_time (nth_nat 1 x)
+  + nth_nat_IMP_Minus_time 2 x +  atomExp_to_constant_IMP_Minus_time (nth_nat 2 x)
+  + IMP_Minus_fst_nat_time (x - 1) + 11" 
+
+lemma Seq: "\<lbrakk>(c1,s1) \<Rightarrow>\<^bsup> x \<^esup> s2;  (c2,s2) \<Rightarrow>\<^bsup> y \<^esup> s3 \<rbrakk> \<Longrightarrow> (c1;;c2, s1) \<Rightarrow>\<^bsup> x + y \<^esup> s3"
+  by auto
+
+lemma aexp_max_constant_IMP_Minus_correct:
+  "(aexp_max_constant_IMP_Minus, s) 
+    \<Rightarrow>\<^bsup>aexp_max_constant_IMP_Minus_time (s ''a'')\<^esup>
+    s(''a'' := 0,
+      ''b'' := 0,
+      ''c'' := 0,
+      ''fst_nat'' := 0,
+      ''snd_nat'' := 0,
+      ''nth_nat'' := 0,
+      ''atomExp_to_constant'' := 0,
+      ''aexp_max_constant'' := aexp_max_constant_tail (s ''a''))"
+  unfolding aexp_max_constant_IMP_Minus_def aexp_max_constant_IMP_Minus_time_def
+  apply(cases "3 - fst_nat (s ''a'' - Suc 0)"; cases "fst_nat (s ''a'' - Suc 0)")
+     apply simp
+  apply(fastforce simp: numeral_eq_Suc hd_nat_def 
+        intro!: terminates_in_time_state_intro[OF Seq]
+        atomExp_to_constant_IMP_Minus_correct
+        nth_nat_IMP_Minus_correct
+        IMP_Minus_max_a_min_b_correct
+        IMP_Minus_fst_nat_correct)
+  (*apply(fastforce simp: numeral_eq_Suc hd_nat_def 
+        intro!: terminates_in_time_state_intro[OF Seq]
+        atomExp_to_constant_IMP_Minus_correct
+        nth_nat_IMP_Minus_correct
+        IMP_Minus_max_a_min_b_correct
+        IMP_Minus_fst_nat_correct)*)
+  subgoal
+    by(fastforce simp: numeral_eq_Suc hd_nat_def 
+        intro!: terminates_in_time_state_intro[OF Seq]
+        atomExp_to_constant_IMP_Minus_correct
+        nth_nat_IMP_Minus_correct
+        IMP_Minus_max_a_min_b_correct
+        IMP_Minus_fst_nat_correct)
+  subgoal
+    by(fastforce simp: numeral_eq_Suc hd_nat_def 
+        intro!: terminates_in_time_state_intro[OF Seq]
+        atomExp_to_constant_IMP_Minus_correct
+        nth_nat_IMP_Minus_correct
+        IMP_Minus_max_a_min_b_correct
+        IMP_Minus_fst_nat_correct)
+  done
+
+
+end
